src/syntax/FStarC.Syntax.DsEnv.fsti
@@ -40,6 +40,7 @@ type record_or_dc = {
 
 val env : Type0
 val dsenv_hooks : Type0
+val parsing_data_for_scope (e:env) : list FStarC.Parser.Dep.parsing_data_elt
 val with_restored_scope (e:env) (f: env -> 'a & env) : 'a & env
 
 instance val showable_env : showable env
